\title 4.2-1

\\
let \quad A = \begin{bmatrix}
 1 & 3\\
 7 & 5
\end{bmatrix} B = \begin{bmatrix}
 6 & 8\\
 4 & 2
\end{bmatrix}
\\
\\
S_{1} = B_{12} - B_{22} = 8 - 2 = 6 \\
S_{2} = A_{11} + A_{12} = 1 + 3 = 4 \\
S_{3} = A_{21} + A_{22} = 7 + 5 = 12 \\
S_{4} = B_{21} - B_{11} = 4 - 6 = -2 \\
S_{5} = A_{11} + A_{22} = 1 + 5 = 6 \\
S_{6} = B_{11} + B_{22} = 6 + 2 = 8 \\
S_{7} = A_{12} - A_{22} = 3 - 5 = -2 \\
S_{8} = B_{21} + B_{22} = 4 + 2 = 6 \\
S_{9} = A_{11} - A_{21} = 1 - 7 = -6 \\
S_{10} = B_{11} + B_{12} = 6 + 8 = 14

\\
P_{1} = A_{11} \cdot S_{1} = \begin{bmatrix}
1
\end{bmatrix} \times \begin{bmatrix}
6
\end{bmatrix} = \begin{bmatrix}
6
\end{bmatrix} \\\\
P_{2} = S_{2} \cdot B_{22} = \begin{bmatrix}
4
\end{bmatrix} \times \begin{bmatrix}
2
\end{bmatrix} = \begin{bmatrix}
8
\end{bmatrix} \\\\
P_{3} = S_{3} \cdot B_{11} = \begin{bmatrix}
12
\end{bmatrix} \times \begin{bmatrix}
6
\end{bmatrix} = \begin{bmatrix}
72
\end{bmatrix} \\\\
P_{4} = A_{22} \cdot S_{4} = \begin{bmatrix}
5
\end{bmatrix} \times \begin{bmatrix}
-2
\end{bmatrix} = \begin{bmatrix}
-10
\end{bmatrix} \\\\
P_{5} = S_5 \cdot S_6 = \begin{bmatrix}
6
\end{bmatrix} \times \begin{bmatrix}
8
\end{bmatrix} = \begin{bmatrix}
48
\end{bmatrix} \\\\

P_{6} = S_{7} \cdot S_{8} = \begin{bmatrix}
-2
\end{bmatrix} \times \begin{bmatrix}
6
\end{bmatrix} = \begin{bmatrix}
-12
\end{bmatrix} \\\\
P_{7} = S_{9} \cdot S_{10} = \begin{bmatrix}
-6
\end{bmatrix} \times \begin{bmatrix}
14
\end{bmatrix} = \begin{bmatrix}
-84
\end{bmatrix} \\

\\
C_{11} = P_{5} + P_{4} - P_{2} + P_{6} = \begin{bmatrix}48\end{bmatrix} - \begin{bmatrix}48\end{bmatrix} - \begin{bmatrix}8\end{bmatrix} - \begin{bmatrix}12\end{bmatrix} = \begin{bmatrix}18\end{bmatrix} \\\\
C_{12} = P_{1} + P_{2} = \begin{bmatrix}6\end{bmatrix} + \begin{bmatrix}8\end{bmatrix} = \begin{bmatrix}14\end{bmatrix} \\\\
C_{21} = P_{3} + P_{4} = \begin{bmatrix}72\end{bmatrix} + \begin{bmatrix}-10\end{bmatrix} = \begin{bmatrix}62\end{bmatrix} \\\\
C_{22} = P_{5} + P_{1} - P_{3} + P_{7} = \begin{bmatrix}48\end{bmatrix} + \begin{bmatrix}6\end{bmatrix} - \begin{bmatrix}72\end{bmatrix} - \begin{bmatrix}-84\end{bmatrix} = \begin{bmatrix}66\end{bmatrix} \\\\
\therefore C = \begin{bmatrix}
18 & 14 \\
62 & 66
\end{bmatrix}
