# 3.1

## 3.1-1
* Q

![](https://github.com/KnewHow/FPAlgorithms/blob/master/problem-solution/chapter03-growthOfFunction/img/3.1-1-q.png?raw=true)
* A

We knew that 2(f(n) + g(n)) =< 2max(f(n), g(n)) => .5(f(n) + g(n)) =< max(f(n) + g(n))

We also knew max(f(n) + g(n)) <= max(f(n) + g(n)) + min(f(n) + g(n)) = f(n) + g(n)

So, the 0.5(f(n) + g(n)) =< max(f(n) + g(n)) <= f(n) + g(n)

c1 is 0.5 and c2 is 1.

## 3.1-2

* Q

![](https://github.com/KnewHow/FPAlgorithms/blob/master/problem-solution/chapter03-growthOfFunction/img/3.1-2-q.png?raw=true)

* A

![](https://github.com/KnewHow/FPAlgorithms/blob/master/problem-solution/chapter03-growthOfFunction/img/3.1-2-a.png?raw=true)

## 3.1-3

*  Q
Explain why the statement, “The running time of algorithm A is at least O(n^2)” is meaningless.
*  A
O-notation is defining a upper bound, but `at least` is defining a lower bound, you can say `at least n^2`, but don't say `at least O(n^2)`

## 3.1-4

*  Q
Is 2^(n+1) = O(2^n)? Is 2^(2n) = O(2^n)

*  A

2^(n+1) = 2 * 2^2 => O(2^n) is right. Howover 2^(2n) = 4^n >=  O(2^2), So the 2^(2n) != O(2^n)

## 3.1-5

* Q
Prove Theorem 3.1. For any two functions f(n) and g(n), we have f(n) = Θ(g(n)) if and only if f(n) = O(g(n)) and f(n) = Ω(g(n)).
* A
if f(n) = Ω(g(n)), so f(n) >= c1 * g(n)
if f(n) = O(g(n)), so 0 <= f(n) <= c2 * g(n), So
c1 * g(n) =< f(n) =< c2 * g(n), So f(n) = Θ(n)

## 3.1-6

*  Q
Prove that the running time of an algorithm is Θ(g(n)) if and only if its worst-case
running time is O(g(n)) and its best-case running time is Ω(g(n)).

*  A
we define the running time is f(n), so we can get following from question:

c1 * g(n) <= f(n) <= c2 * g(n), So the running time is Θ(g(n))

## 3.1-7

*  Q
Prove that o(g(n)) ∩ w(g(n)) is the empty set.

*  A
f(n) = o(g(n)) is like a < b, but f(n) < w(g(n)) is like a > c, so b ∩ c is empty.

## 3.1-8

*  Q

![](https://github.com/KnewHow/FPAlgorithms/blob/master/problem-solution/chapter03-growthOfFunction/img/3.1-8-q.png?raw=true)
*  A

Ω(g(n,m)) = { f(n,m) : there exsit positive constants c n0, and m0
                     such that 0 <= c * g(n,m) <= f(n,m)
                     for all n >= n0 and m >= m0}


Some solution refer:http://sites.math.rutgers.edu/~ajl213/CLRS/Ch3.pdf
