# 3.2

## 3.2-1

*  Q
Show that if `f(n)` and `g(n)` are monotonically increasing functions, then so are
the functions `f(n) + g(n)` and `f(g(n))` and if f(n) and g(n) are in addition
nonnegative, then `f(n) * g(n)` is monotonically increasing.

*  A

when `n2 >= n1`, so `(f(n2) + g(n2)) - (f(n1) - g(n1))` = `f(n2) - f(n1) + g(n2) - g(n1) >=0` . So the `f(n) + g(n)` is monotonically increasing.

when `n2 >= n1`, so `f(g(n2)) - f(g(n1)) = f(k2) - f(k1)` We let `g(n1) = k1` and `g(n2) = k2` so  `k2 >= k1`. So `f(k2) - f(k1) >=0` => f(g(n)) is monotonically increasing.

when `n2 >= n1` and `f(n) >= 0` and `g(n) >= 0`, so `f(n2)*g(n2) - f(n1)*g(n1) = f(n2)(g(n2)-g(n1))`

when `n2 >= n1` so `f(n2)g(n2) - f(n1)g(n1)` = `f(n2) * (g(n2) - g(n1)) + (f(n2) - f(n1)) * g(n1)`
we knew `f(n)` and `g(n)` are in addition nonnegative, so `f(n) * g(n)` is monotonically increasing.

## 3.2-2

*  Q
Prove equation (3.16) => `a^(log(b)(c)) = c^(log(b)(a))`

*  A
`a^log((b)(c)) = a^(log(a)(c) / log(a)(b)) = c^(1 / log(a)(b)) = c^log(b)(a)`

## 3.2-3

*  Q
Prove equation (3.19). Also prove that n! = w(2^n) and n! = o(n^n)

*  A

1.

![](https://github.com/KnewHow/FPAlgorithms/blob/master/problem-solution/chapter03-growthOfFunction/img/3.2-3-1-a.gif?raw=true)

2.

![](https://github.com/KnewHow/FPAlgorithms/blob/master/problem-solution/chapter03-growthOfFunction/img/3.2-3-2-a.gif?raw=true)

3.

![](https://github.com/KnewHow/FPAlgorithms/blob/master/problem-solution/chapter03-growthOfFunction/img/3.2-3-3-a.gif?raw=true)

## 3.2-4

*  Q
 ![](https://github.com/KnewHow/FPAlgorithms/blob/master/problem-solution/chapter03-growthOfFunction/img/3.2-4-q.png?raw=true)
