\\
let \quad A_{m \times n} = \begin{bmatrix}
 a_{11}&   a_{12} & ... & a_{1n}\\
 a_{21}&   a_{22} & ... & a_{2n}\\
 ... & ... & ... & ... \\
 a_{m1}&   a_{m2} & ... & a_{mn}
\end{bmatrix}
\\
\\\\
let \quad B_{n \times p} = \begin{bmatrix}
 b_{11}&   b_{12} & ... & b_{1p}\\
 b_{21}&   b_{22} & ... & b_{2p}\\
 ... & ... & ... & ... \\
 b_{n1}&   b_{n2} & ... & b_{np}
\end{bmatrix}
\\
\therefore\quad C_{m \times p} = A \times B = \begin{bmatrix}
 \sum_{d=1}^{n}a_{1d}b_{d1} & \sum_{d=1}^{n}a_{1d}b_{d2} & ... & \sum_{d=1}^{n}a_{1d}b_{dp}\\ \\
 \sum_{d=1}^{n}a_{2d}b_{d1} & \sum_{d=1}^{n}a_{2d}b_{d2} & ... & \sum_{d=1}^{n}a_{2d}b_{dp}\\  \\
 ... & ... & ... & ... \\
 \sum_{d=1}^{n}a_{md}b_{d1} & \sum_{d=1}^{n}a_{md}b_{d2} & ... & \sum_{d=1}^{n}a_{md}b_{dp}\\
\end{bmatrix}
\\\\
\\
\therefore \quad C^T_{p \times m} = \begin{bmatrix}
 \sum_{d=1}^{n}a_{1d}b_{d1}& \sum_{d=1}^{n}a_{2d}b_{d1} & ... &\sum_{d=1}^{n}a_{md}b_{d1}  \\\\
 \sum_{d=1}^{n}a_{1d}b_{d2} & \sum_{d=1}^{n}a_{2d}b_{d2} & ... &\sum_{d=1}^{n}a_{md}b_{d2} \\
 ...& ... & ... & ...\\
 \sum_{d=1}^{n}a_{1d}b_{dp} & \sum_{d=1}^{n}a_{2d}b_{dp} & ... & \sum_{d=1}^{n}a_{md}b_{dp}
\end{bmatrix}
\\
\\
\therefore \quad A^T_{n \times m} = \begin{bmatrix}
a_{11} & a_{21}  & ... &  a_{m1}\\
a_{12}& a_{22} & ... & a_{m2} \\
...& ... & ... & ... \\
a_{1n}& a_{2n} & ... & a_{mn}
\end{bmatrix}
\\\\
\\
\therefore \quad B^T_{p \times n} = \begin{bmatrix}
b_{11} & b_{21}  & ... &  b_{n1}\\
b_{12}& b_{22} & ... & b_{n2} \\
...& ... & ... & ... \\
b_{1p}& b_{2p} & ... & b_{np}
\end{bmatrix}
\\\\
\\
\therefore B^T_{p \times n}A^T_{n \times m} = D_{p \times m} = \begin{bmatrix}
\sum_{d=1}^{n}b_{d1}a_{1d} & \sum_{d=1}^{n}b_{d1}a_{2d} & ... & \sum_{d=1}^{n}b_{d1}a_{md} \\\\
\sum_{d=1}^{n}b_{d2}a_{1d} & \sum_{d=1}^{n}b_{d2}a_{2d} & ... & \sum_{d=1}^{n}b_{d2}a_{md} \\
 ... & ... & ... & ... \\
\sum_{d=1}^{n}b_{dp}a_{1d} & \sum_{d=1}^{n}b_{dp}a_{2d} & ... & \sum_{d=1}^{n}b_{dp}a_{md} \\
\end{bmatrix}
