# 4.3

## 4.3-1

*  Q

Show that the solution of `T(n) = T(n-1) + n` is ![](http://latex.codecogs.com/gif.latex?O(n^2))

*  A

![](https://github.com/KnewHow/FPAlgorithms/blob/master/problem-solution/chapter04-divideAndConquer/img/4.3-1-a.gif?raw=true)


## 4.3-2

*  Q

![](https://github.com/KnewHow/FPAlgorithms/blob/master/problem-solution/chapter04-divideAndConquer/img/4.3-2-q.png?raw=true)

*  A

![](https://github.com/KnewHow/FPAlgorithms/blob/master/problem-solution/chapter04-divideAndConquer/img/4.3-2-a.gif?raw=true)

## 4.3-3

*  Q

![](https://github.com/KnewHow/FPAlgorithms/blob/master/problem-solution/chapter04-divideAndConquer/img/4.3-3-q.png?raw=true)

*  A

![](https://github.com/KnewHow/FPAlgorithms/blob/master/problem-solution/chapter04-divideAndConquer/img/4.3-3-a.png?raw=true)
